more changes to box, Indexing WIP

examples/crypto/cryptobox/Box.DH.fst
@@ -18,6 +18,9 @@ open Box.Indexing
 open Box.PlainDH
 open Box.Flags
 
+module MR = FStar.Monotonic.RRef
+module MM = MonotoneMap
+
 
 assume val dh_share_size : nat
 assume val dh_exponent_size : nat
@@ -30,15 +33,28 @@ type keysize = aeadKeySize AES_128_GCM
 type aes_key = lbytes keysize (* = b:bytes{B.length b = keysize} *)
 
 
-noeq type entry (i:id) = 
-  | DH_entry: ent_i:id -> ent_share:dh_share -> ent_key:PlainDH.key{AE.get_index ent_key = (i,ent_i) /\ ae_honest (i,ent_i)} -> entry i
+//noeq type entry (i:id) = 
+//  | DH_entry: ent_i:id -> ent_share:dh_share -> ent_key:PlainDH.key{AE.get_index ent_key = (i,ent_i) /\ ae_honest (i,ent_i)} -> entry i
 
 
-type log_t (i:id) (r:rid) = m_rref r (seq (entry i)) grows
+(*
+  Setting up a global log for AE.keys indexed by the ids of the public and private key involved.
+*)
+private type range = fun (k_id:ae_id) -> k:PlainDH.key{(AE.get_index k = k_id) || (AE.get_index k = (snd k_id,fst k_id))}
+private let inv (f:MM.map' (ae_id) range) = True
+//type log_t (i:id) (r:rid) = m_rref r (seq (entry i)) grows
+private let ae_key_log = MM.alloc #root #ae_id #range #inv
+private let (ae_key_region:MR.rid) = new_region root
 
 
+//noeq abstract type dh_pkey = 
+//  | DH_pkey:  #pk_id:id -> #region:rid ->rawpk:dh_share -> log:log_t pk_id region -> dh_pkey
+//
+//
+//noeq abstract type dh_skey =
+//  | DH_skey: #sk_id:id -> rawsk:dh_exponent -> pk:dh_pkey{pk.pk_id=sk_id} -> dh_skey 
 noeq abstract type dh_pkey = 
-  | DH_pkey:  #pk_id:id -> #region:rid ->rawpk:dh_share -> log:log_t pk_id region -> dh_pkey
+  | DH_pkey:  #pk_id:id -> rawpk:dh_share -> dh_pkey
 
 
 noeq abstract type dh_skey =
@@ -54,17 +70,15 @@ val pk_get_rawpk: pk:dh_pkey -> Tot (raw:dh_share{raw=pk.rawpk})
 let pk_get_rawpk pk =
   pk.rawpk
 
-val keygen: #i:id -> (parent:rid) -> ST (dh_pair:(k:dh_pkey{k.pk_id=i}) * (k:dh_skey{k.sk_id=i}))
+val keygen: #i:id -> ST (dh_pair:(k:dh_pkey{k.pk_id=i}) * (k:dh_skey{k.sk_id=i}))
   (requires (fun h -> True))
   (ensures (fun h0 k h1 -> True
 //  let (pk,sk) = k in
 //  safe_key_gen parent pk h0 h1
   ))
-let keygen #i parent =
-  let region = new_region parent in
-  let log = alloc_mref_seq region createEmpty in
+let keygen #i =
   let dh_share,dh_exponent = dh_gen_key() in
-  let dh_pk = DH_pkey #i #region dh_share log in
+  let dh_pk = DH_pkey #i dh_share in
   let dh_sk = DH_skey #i dh_exponent dh_pk in
   dh_pk,dh_sk
 
@@ -74,74 +88,69 @@ let keygen #i parent =
 *)
 assume val dh_exponentiate: dh_share -> dh_exponent -> Tot aes_key
 
-type safe_log_append pk entry h0 h1 =
-    modifies_one pk.region h0 h1 
-    /\ m_contains pk.log h1
-    /\ m_sel h1 pk.log == snoc (m_sel h0 pk.log) entry
-    /\ witnessed (at_least (Seq.length (m_sel h0 pk.log)) entry pk.log)
+//type safe_log_append pk entry h0 h1 =
+//    modifies_one pk.region h0 h1 
+//    /\ m_contains pk.log h1
+//    /\ m_sel h1 pk.log == snoc (m_sel h0 pk.log) entry
+//    /\ witnessed (at_least (Seq.length (m_sel h0 pk.log)) entry pk.log)
 
 (**
    Helper function to look entries up in a log.
 *)
-val equal_share: sk_id:id -> pk_id:id -> dh_sh:dh_share -> e:entry sk_id -> Tot bool
-let equal_share sk_id pk_id dh_sh e =
-  match e with 
-  | DH_entry ent_i ent_share _ -> ent_i=pk_id && ent_share = dh_sh
+
+//val equal_share: sk_id:id -> pk_id:id -> dh_sh:dh_share -> e:entry sk_id -> Tot bool
+//let equal_share sk_id pk_id dh_sh e =
+//  match e with 
+//  | DH_entry ent_i ent_share _ -> ent_i=pk_id && ent_share = dh_sh
 
 (**
    If we prf_odh is true, the output of this function is random, if both 
    share and exponent are honest.
 *)
-val prf_odh_snd: sk:dh_skey -> pk:dh_pkey -> ST (PlainDH.key)
+val prf_odh: sk:dh_skey -> pk:dh_pkey -> ST (PlainDH.key)
   ( requires (fun _ -> True))
   ( ensures (fun _ k _ -> 
     (Box.AE.get_index k = (sk.sk_id, pk.pk_id)) || (Box.AE.get_index k = (pk.pk_id, sk.sk_id))
   ))
-let prf_odh_snd dh_snd_sk dh_rcv_pk =
-  let pk_id = dh_rcv_pk.pk_id in
-  let sk_id = dh_snd_sk.sk_id in
+let prf_odh dh_sk dh_pk =
+  let pk_id = dh_pk.pk_id in
+  let sk_id = dh_sk.sk_id in
   let i = pk_id, sk_id in
   let ae_honest_i = ae_honestST i in
   if ae_honest_i && prf_odh then
-    let rcv_log = m_read dh_rcv_pk.log in
-    let snd_log = m_read dh_snd_sk.pk.log in
-    let rcv_entry = seq_find (equal_share pk_id sk_id dh_rcv_pk.rawpk) rcv_log in
-    let snd_entry = seq_find (equal_share sk_id pk_id dh_snd_sk.pk.rawpk) snd_log in
-    match rcv_entry with
-    | Some (DH_entry _ _ k') -> k'
+    (MR.m_recall ae_key_log;
+    let entry = MM.lookup ae_key_log i in
+    match entry with
+    | Some  k' -> k'
     | None -> 
-      match snd_entry with
-      | Some (DH_entry _ _ k') -> k'
-      | None -> 
-      let k' = PlainDH.keygen i dh_rcv_pk.region in
-      write_at_end dh_rcv_pk.log (DH_entry sk_id dh_snd_sk.pk.rawpk k');
-      write_at_end dh_snd_sk.pk.log (DH_entry pk_id dh_rcv_pk.rawpk k');
-      k'
+      let k' = PlainDH.keygen i ae_key_region in
+      MM.extend ae_key_log i k';
+      k')
   else
-    let real_k = dh_exponentiate dh_rcv_pk.rawpk dh_snd_sk.rawsk in
-    let k=PlainDH.coerce_key i dh_rcv_pk.region real_k in
+    let real_k = dh_exponentiate dh_pk.rawpk dh_sk.rawsk in
+    let k=PlainDH.coerce_key i ae_key_region real_k in
     k
 
 
 
-val prf_odh_rcv: #(sk_id:id) -> dh_sk:dh_skey{dh_sk.sk_id=sk_id} -> #(pk_id:id) -> dh_snd_pk:dh_pkey{dh_snd_pk.pk_id=pk_id} ->  St (k:PlainDH.key{AE.get_index k = (sk_id,pk_id)}
-)
-let prf_odh_rcv #sk_id dh_rcv_sk #pk_id dh_snd_pk  =
-  let honest_i = ae_honestST (sk_id, pk_id) in
-  if honest_i && prf_odh then
-    let log = m_read dh_rcv_sk.pk.log in
-    let e = seq_find (equal_share sk_id pk_id dh_snd_pk.rawpk) log in
-    match e with
-    | Some (DH_entry _ _ k') -> k'
-    | None -> 
-      let i = sk_id,pk_id in
-      let k = PlainDH.keygen i dh_rcv_sk.pk.region in
-      k
-//      let i = sk_id,dishonestId() in
-//      let raw_k = dh_exponentiate dh_snd_pk.rawpk dh_rcv_sk.rawsk in
-//      admit ();
-//      PlainDH.coerce_key i dh_rcv_sk.pk.region raw_k
-  else
-    let i =  sk_id,pk_id in
-    let raw_k = dh_exponentiate dh_snd_pk.rawpk dh_rcv_sk.rawsk in
-    PlainDH.coerce_key i dh_rcv_sk.pk.region raw_k
+//val prf_odh_rcv: #(sk_id:id) -> dh_sk:dh_skey{dh_sk.sk_id=sk_id} -> #(pk_id:id) -> dh_snd_pk:dh_pkey{dh_snd_pk.pk_id=pk_id} ->  St (k:PlainDH.key{AE.get_index k = (sk_id,pk_id)}
+//)
+//let prf_odh_rcv #sk_id dh_rcv_sk #pk_id dh_snd_pk  =
+//  let honest_i = ae_honestST (sk_id, pk_id) in
+//  if honest_i && prf_odh then
+//    let log = m_read dh_rcv_sk.pk.log in
+//    let e = seq_find (equal_share sk_id pk_id dh_snd_pk.rawpk) log in
+//    match e with
+//    | Some (DH_entry _ _ k') -> k'
+//    | None -> 
+//      let i = sk_id,pk_id in
+//      let k = PlainDH.keygen i dh_rcv_sk.pk.region in
+//      k
+////      let i = sk_id,dishonestId() in
+////      let raw_k = dh_exponentiate dh_snd_pk.rawpk dh_rcv_sk.rawsk in
+////      admit ();
+////      PlainDH.coerce_key i dh_rcv_sk.pk.region raw_k
+//  else
+//    let i =  sk_id,pk_id in
+//    let raw_k = dh_exponentiate dh_snd_pk.rawpk dh_rcv_sk.rawsk in
+//    PlainDH.coerce_key i dh_rcv_sk.pk.region raw_k
